@prefix mwo: <http://example.org/#> .
@base        <http://example.org/> .
@prefix bibo: <http://purl.org/ontology/bibo/> .
@prefix daia: <http://purl.org/ontology/daia/> .
@prefix dct:  <http://purl.org/dc/terms/> .
@prefix dso:  <http://purl.org/ontology/dso#> .
@prefix ecpo: <http://purl.org/ontology/ecpo#> .
@prefix owl:  <http://www.w3.org/2002/07/owl#> .
@prefix rdfs: <http://www.w3.org/2000/01/rdf-schema#> .
@prefix vann: <http://purl.org/vocab/vann/> .
@prefix xsd:  <http://www.w3.org/2001/XMLSchema#> .
<> a owl:Ontology ;
    rdfs:label "Moving Wall Ontology (MWO)" ;
    vann:preferredNamespacePrefix "mwo" .
dso:DocumentService a owl:Class ;
    rdfs:label "DocumentService" ;
    rdfs:isDefinedBy <http://purl.org/ontology/dso> .
mwo:numVolumes a owl:DatatypeProperty ;
    rdfs:label "number of volumes" ;
    rdfs:comment "The number of volumes that are included in or excluded from the DocumentService." ;
    rdfs:domain dso:DocumentService ;
    rdfs:range xsd:integer .
mwo:numIssues a owl:DatatypeProperty ;
    rdfs:label "number of issues" ;
    rdfs:comment "The number of issues that are included in or excluded from the DocumentService." ;
    rdfs:domain dso:DocumentService ;
    rdfs:range xsd:integer .
mwo:time a owl:DatatypeProperty ;
    rdfs:label "period of time" ;
    rdfs:comment "A part of the item expressed through a period of time which is included in or excluded from the DocumentService." ;
    rdfs:domain dso:DocumentService ;
    rdfs:range xsd:duration .
