@prefix rdf: <http://www.w3.org/1999/02/22-rdf-syntax-ns#> .
@prefix mwo: <http://example.org/#> .
@prefix bibo: <http://purl.org/ontology/bibo/> .
@prefix daia: <http://purl.org/ontology/daia/> .
@prefix dct: <http://purl.org/dc/terms/> .
@prefix dso: <http://purl.org/ontology/dso#> .
@prefix ecpo: <http://purl.org/ontology/ecpo#> .
@prefix owl: <http://www.w3.org/2002/07/owl#> .
@prefix rdfs: <http://www.w3.org/2000/01/rdf-schema#> .
@prefix vann: <http://purl.org/vocab/vann/> .
@prefix xsd: <http://www.w3.org/2001/XMLSchema#> .

<http://example.org/>
    vann:preferredNamespacePrefix "mwo" ;
    a owl:Ontology ;
    rdfs:label "Moving Wall Ontology (MWO)" .

mwo:numIssues
    a owl:DatatypeProperty ;
    rdfs:comment "The number of issues that are included in or excluded from the DocumentService." ;
    rdfs:domain dso:DocumentService ;
    rdfs:label "number of issues" ;
    rdfs:range xsd:integer .

mwo:numVolumes
    a owl:DatatypeProperty ;
    rdfs:comment "The number of volumes that are included in or excluded from the DocumentService." ;
    rdfs:domain dso:DocumentService ;
    rdfs:label "number of volumes" ;
    rdfs:range xsd:integer .

mwo:time
    a owl:DatatypeProperty ;
    rdfs:comment "A part of the item expressed through a period of time which is included in or excluded from the DocumentService." ;
    rdfs:domain dso:DocumentService ;
    rdfs:label "period of time" ;
    rdfs:range xsd:duration .

dso:DocumentService
    a owl:Class ;
    rdfs:isDefinedBy <http://purl.org/ontology/dso> ;
    rdfs:label "DocumentService" .

