@prefix rdf: <http://www.w3.org/1999/02/22-rdf-syntax-ns#> .
@prefix mwo: <http://example.org/#> .
@prefix dso: <http://purl.org/ontology/dso#> .
@prefix ssso: <http://purl.org/ontology/ssso#> .
@prefix owl: <http://www.w3.org/2002/07/owl#> .
@prefix rdfs: <http://www.w3.org/2000/01/rdf-schema#> .
@prefix vann: <http://purl.org/vocab/vann/> .
@prefix xs: <http://www.w3.org/2001/XMLSchema#> .
@prefix dc: <http://purl.org/dc/elements/1.1/> .

<http://example.org/>
    dc:description "A vocabulary to express a limitation to a document service"@en ;
    dc:title "Moving Wall Ontology (MWO)" ;
    vann:preferredNamespacePrefix "mwo" ;
    a owl:Ontology ;
    rdfs:label "Moving Wall Ontology (MWO)" .

mwo:MovingWall
    a owl:Class ;
    rdfs:comment "A moving wall is some obstacle that may limit the use of a ssso:ServiceEvent" ;
    rdfs:label "moving wall" ;
    rdfs:subClassOf ssso:ServiceLimitation, [
        a owl:Class ;
        owl:unionOf ([
                a owl:Restriction ;
                owl:onProperty mwo:numVolumes ;
                owl:someValuesFrom owl:Thing
            ]
            [
                a owl:Restriction ;
                owl:onProperty mwo:numIssues ;
                owl:someValuesFrom owl:Thing
            ]
            [
                a owl:Restriction ;
                owl:onProperty mwo:timePeriod ;
                owl:someValuesFrom owl:Thing
            ]
        )
    ] .

mwo:limitedBy
    a owl:ObjectProperty ;
    rdfs:comment "Relates a dso:DocumentService instance that is limited by a moving wall instance to this service limitation." ;
    rdfs:domain dso:DocumentService ;
    rdfs:label "limited by" ;
    rdfs:range mwo:MovingWall ;
    rdfs:subPropertyOf ssso:limitedBy .

mwo:numIssues
    a owl:DatatypeProperty ;
    rdfs:comment "A limitation to the DocumentService in the form of number of volumes." ;
    rdfs:domain dso:DocumentService ;
    rdfs:label "number of issues" ;
    rdfs:range xs:integer .

mwo:numVolumes
    a owl:DatatypeProperty ;
    rdfs:comment "A limitation to the DocumentService in the form of number of volumes." ;
    rdfs:domain dso:DocumentService ;
    rdfs:label "number of volumes" ;
    rdfs:range xs:integer .

mwo:timePeriod
    a owl:DatatypeProperty ;
    rdfs:comment "A limitation to the DocumentService in the form of a period of time." ;
    rdfs:domain dso:DocumentService ;
    rdfs:label "period of time" ;
    rdfs:range xs:duration .

